theories/zoo_parabs/ws_hub_fifo.v
@@ -1,16 +1,753 @@
 From zoo Require Import
   prelude.
+From zoo.common Require Import
+  countable.
+From zoo.iris.bi Require Import
+  big_op.
+From zoo.iris.base_logic Require Import
+  lib.twins
+  lib.excl.
 From zoo.language Require Import
   notations.
 From zoo.diaframe Require Import
   diaframe.
+From zoo_std Require Import
+  option
+  domain.
+From zoo_saturn Require Import
+  mpmc_queue_1.
 From zoo_parabs Require Export
   base
   ws_hub_fifo__code.
 From zoo_parabs Require Import
-  ws_hub_fifo__types.
+  ws_hub_fifo__types
+  ws_deques_public
+  waiters.
 From zoo Require Import
   options.
+
+Implicit Types b yield killed : bool.
+Implicit Types l : location.
+Implicit Types v t until pred : val.
+Implicit Types ws : list val.
+Implicit Types vs : gmultiset val.
+
+Class WsHubFifoG Σ `{zoo_G : !ZooG Σ} := {
+  #[local] ws_hub_fifo_G_queue_G :: MpmcQueue1G Σ ;
+  #[local] ws_hub_fifo_G_waiters_G :: WaitersG Σ ;
+  #[local] ws_hub_fifo_G_model_G :: TwinsG Σ (leibnizO (gmultiset val)) ;
+  #[local] ws_hub_fifo_G_owner_G :: ExclG Σ unitO ;
+}.
+
+Definition ws_hub_fifo_Σ := #[
+  mpmc_queue_1_Σ ;
+  waiters_Σ ;
+  twins_Σ (leibnizO (gmultiset val)) ;
+  excl_Σ unitO
+].
+#[global] Instance subG_ws_hub_fifo_Σ Σ `{zoo_G : !ZooG Σ} :
+  subG ws_hub_fifo_Σ Σ →
+  WsHubFifoG Σ.
+Proof.
+  solve_inG.
+Qed.
+
+Section ws_hub_fifo_G.
+  Context `{ws_hub_fifo_G : WsHubFifoG Σ}.
+
+  Record metadata := {
+    metadata_size : nat ;
+    metadata_queue : val ;
+    metadata_waiters : val ;
+    metadata_model : gname ;
+    metadata_owners : list gname ;
+  }.
+  Implicit Types γ : metadata.
+  Implicit Types γ_owners : list gname.
+
+  #[local] Instance metadata_eq_dec : EqDecision metadata :=
+    ltac:(solve_decision).
+  #[local] Instance metadata_countable :
+    Countable metadata.
+  Proof.
+    solve_countable.
+  Qed.
+
+  #[local] Definition model₁' γ_model vs :=
+    twins_twin1 γ_model (DfracOwn 1) vs.
+  #[local] Definition model₁ γ :=
+    model₁' γ.(metadata_model).
+  #[local] Definition model₂' γ_model vs :=
+    twins_twin2 γ_model vs.
+  #[local] Definition model₂ γ vs :=
+    model₂' γ.(metadata_model) vs.
+
+  #[local] Definition owner' γ_owners i : iProp Σ :=
+    ∃ γ_owner,
+    ⌜γ_owners !! i = Some γ_owner⌝ ∗
+    excl γ_owner ().
+  #[local] Definition owner γ i :=
+    owner' γ.(metadata_owners) i.
+  #[local] Instance : CustomIpatFormat "owner_" :=
+    "(
+      %γ_owner{} &
+      %Hlookup{} &
+      Howner{}
+    )".
+
+  #[local] Definition ws_hub_fifo_inv_inner l γ : iProp Σ :=
+    ∃ ws killed,
+    l.[killed] ↦ #killed ∗
+    mpmc_queue_1_model γ.(metadata_queue) ws ∗
+    model₂ γ (list_to_set_disj ws).
+  #[local] Instance : CustomIpatFormat "inv_inner" :=
+    "(
+      %ws &
+      %killed &
+      >Hl_killed &
+      >Hqueue_model &
+      >Hmodel₂
+    )".
+  Definition ws_hub_fifo_inv t ι : iProp Σ :=
+    ∃ l γ,
+    ⌜t = #l⌝ ∗
+    meta l nroot γ ∗
+    l.[size] ↦□ #γ.(metadata_size) ∗
+    l.[queue] ↦□ γ.(metadata_queue) ∗
+    l.[waiters] ↦□ γ.(metadata_waiters) ∗
+    mpmc_queue_1_inv γ.(metadata_queue) (ι.@"queue") ∗
+    waiters_inv γ.(metadata_waiters) ∗
+    inv (ι.@"inv") (ws_hub_fifo_inv_inner l γ).
+  #[local] Instance : CustomIpatFormat "inv" :=
+    "(
+      %l &
+      %γ &
+      -> &
+      #Hmeta &
+      #Hl_size &
+      #Hl_queue &
+      #Hl_waiters &
+      #Hqueue_inv &
+      #Hwaiters_inv &
+      #Hinv
+    )".
+
+  Definition ws_hub_fifo_model t vs : iProp Σ :=
+    ∃ l γ,
+    ⌜t = #l⌝ ∗
+    meta l nroot γ ∗
+    model₁ γ vs.
+  #[local] Instance : CustomIpatFormat "model" :=
+    "(
+      %l_ &
+      %γ_ &
+      %Heq &
+      Hmeta_ &
+      Hmodel₁
+    )".
+
+  Definition ws_hub_fifo_owner t i : iProp Σ :=
+    ∃ l γ,
+    ⌜t = #l⌝ ∗
+    meta l nroot γ ∗
+    owner γ i.
+  #[local] Instance : CustomIpatFormat "owner" :=
+    "(
+      %l{=_} &
+      %γ{=_} &
+      %Heq{} &
+      #Hmeta{=_} &
+      Howner{}
+    )".
+
+  #[global] Instance ws_hub_fifo_model_timeless t vs :
+    Timeless (ws_hub_fifo_model t vs).
+  Proof.
+    apply _.
+  Qed.
+  #[global] Instance ws_hub_fifo_owner_timeless t i :
+    Timeless (ws_hub_fifo_owner t i).
+  Proof.
+    apply _.
+  Qed.
+  #[global] Instance ws_hub_fifo_inv_persistent t ι :
+    Persistent (ws_hub_fifo_inv t ι).
+  Proof.
+    apply _.
+  Qed.
+
+  #[local] Lemma model_alloc :
+    ⊢ |==>
+      ∃ γ_model,
+      model₁' γ_model ∅ ∗
+      model₂' γ_model ∅.
+  Proof.
+    apply twins_alloc'.
+  Qed.
+  #[local] Lemma model_agree γ vs1 vs2 :
+    model₁ γ vs1 -∗
+    model₂ γ vs2 -∗
+    ⌜vs1 = vs2⌝.
+  Proof.
+    apply: twins_agree_L.
+  Qed.
+  #[local] Lemma model_update {γ vs1 vs2} vs :
+    model₁ γ vs1 -∗
+    model₂ γ vs2 ==∗
+      model₁ γ vs ∗
+      model₂ γ vs.
+  Proof.
+    apply twins_update'.
+  Qed.
+
+  #[local] Lemma owner_alloc sz :
+    ⊢ |==>
+      ∃ γ_owners,
+      [∗ list] i ∈ seq 0 sz,
+        owner' γ_owners i.
+  Proof.
+    iAssert (
+      [∗ list] i ∈ seq 0 sz,
+        |==>
+        ∃ γ_owner,
+        excl (excl_G := ws_hub_fifo_G_owner_G) γ_owner ()
+    )%I as "-#H".
+    { iApply big_sepL_intro. iIntros "!> % % _".
+      iApply excl_alloc.
+    }
+    iMod (big_sepL_bupd with "H") as "H".
+    iDestruct (big_sepL_exists with "H") as "(%γ_owners & _ & H)".
+    iDestruct (big_sepL2_retract_r with "H") as "(_ & H)".
+    iDestruct (big_sepL_seq_index_2 with "H") as "H".
+    { rewrite length_seq //. }
+    iSteps.
+  Qed.
+  #[local] Lemma owner_exclusive γ i :
+    owner γ i -∗
+    owner γ i -∗
+    False.
+  Proof.
+    iIntros "(:owner_ =1) (:owner_ =2)". simplify.
+    iApply (excl_exclusive with "Howner1 Howner2").
+  Qed.
+
+  Opaque owner'.
+
+  Lemma ws_hub_fifo_owner_exclusive t i :
+    ws_hub_fifo_owner t i -∗
+    ws_hub_fifo_owner t i -∗
+    False.
+  Proof.
+    iIntros "(:owner =1) (:owner =2)". simplify.
+    iDestruct (meta_agree with "Hmeta1 Hmeta2") as %->.
+    iApply (owner_exclusive with "Howner1 Howner2").
+  Qed.
+
+  Lemma ws_hub_fifo_create_spec ι sz :
+    (0 ≤ sz)%Z →
+    {{{
+      True
+    }}}
+      ws_hub_fifo_create #sz
+    {{{ t,
+      RET t;
+      ws_hub_fifo_inv t ι ∗
+      ws_hub_fifo_model t ∅ ∗
+      [∗ list] i ∈ seq 0 ₊sz,
+        ws_hub_fifo_owner t i
+    }}}.
+  Proof.
+    iIntros "%Hsz %Φ _ HΦ".
+
+    wp_rec.
+    wp_apply (waiters_create_spec with "[//]") as (waiters) "#Hwaiters_inv".
+    wp_apply (mpmc_queue_1_create_spec with "[//]") as (queue) "(#Hqueue_inv & Hqueue_model)".
+    wp_block l as "Hmeta" "(Hl_size & Hl_queue & Hl_waiters & Hl_killed & _)".
+    iMod (pointsto_persist with "Hl_size") as "#Hl_size".
+    iMod (pointsto_persist with "Hl_queue") as "#Hl_queue".
+    iMod (pointsto_persist with "Hl_waiters") as "#Hl_waiters".
+
+    iMod model_alloc as "(%γ_model & Hmodel₁ & Hmodel₂)".
+    iMod owner_alloc as "(%γ_owners & Howners)".
+
+    pose γ := {|
+      metadata_size := ₊sz ;
+      metadata_queue := queue ;
+      metadata_waiters := waiters ;
+      metadata_model := γ_model ;
+      metadata_owners := γ_owners ;
+    |}.
+    iMod (meta_set _ _ γ with "Hmeta") as "#Hmeta"; first done.
+
+    iApply "HΦ".
+    iSplitR "Hmodel₁ Howners". { iSteps. rewrite Z2Nat.id //. iSteps. }
+    iSteps.
+    iApply (big_sepL_impl with "Howners"). iSteps.
+  Qed.
+
+  #[local] Lemma ws_hub_fifo_size_spec t ι :
+    {{{
+      ws_hub_fifo_inv t ι
+    }}}
+      ws_hub_fifo_size t
+    {{{ (sz : nat),
+      RET #sz;
+      True
+    }}}.
+  Proof.
+    iSteps.
+  Qed.
+
+  Lemma ws_hub_fifo_killed_spec t ι :
+    {{{
+      ws_hub_fifo_inv t ι
+    }}}
+      ws_hub_fifo_killed t
+    {{{ killed,
+      RET #killed;
+      True
+    }}}.
+  Proof.
+    iSteps.
+  Qed.
+
+  #[local] Lemma ws_hub_fifo_notify_spec t ι :
+    {{{
+      ws_hub_fifo_inv t ι
+    }}}
+      ws_hub_fifo_notify t
+    {{{
+      RET ();
+      True
+    }}}.
+  Proof.
+    iIntros "%Φ (:inv) HΦ".
+
+    wp_rec. wp_load.
+    wp_apply (waiters_notify_spec with "Hwaiters_inv HΦ").
+  Qed.
+
+  #[local] Lemma ws_hub_fifo_notify_all_spec t ι :
+    {{{
+      ws_hub_fifo_inv t ι
+    }}}
+      ws_hub_fifo_notify_all t
+    {{{
+      RET ();
+      True
+    }}}.
+  Proof.
+    iIntros "%Φ (:inv) HΦ".
+
+    wp_rec.
+    wp_apply (ws_hub_fifo_size_spec) as (sz) "_"; first iSteps.
+    wp_load.
+    wp_apply (waiters_notify_many_spec with "Hwaiters_inv HΦ"); first lia.
+  Qed.
+
+  Lemma ws_hub_fifo_push_spec t ι i i_ v :
+    i = ⁺i_ →
+    <<<
+      ws_hub_fifo_inv t ι ∗
+      ws_hub_fifo_owner t i_
+    | ∀∀ vs,
+      ws_hub_fifo_model t vs
+    >>>
+      ws_hub_fifo_push t #i v @ ↑ι
+    <<<
+      ws_hub_fifo_model t ({[+v+]} ⊎ vs)
+    | RET ();
+      ws_hub_fifo_owner t i_
+    >>>.
+  Proof.
+    iIntros (->) "%Φ ((:inv) & Howner) HΦ".
+
+    wp_rec. wp_load.
+
+    awp_apply (mpmc_queue_1_push_spec with "Hqueue_inv") without "Howner".
+    iInv "Hinv" as "(:inv_inner)".
+    iApply (aacc_aupd_commit with "HΦ"); first solve_ndisj. iIntros "%vs (:model)". injection Heq as <-.
+    iDestruct (meta_agree with "Hmeta Hmeta_") as %<-. iClear "Hmeta_".
+    iDestruct (model_agree with "Hmodel₁ Hmodel₂") as %->.
+    iAaccIntro with "Hqueue_model"; first iSteps. iIntros "Hqueue_model".
+    iMod (model_update (list_to_set_disj $ ws ++ [v]) with "Hmodel₁ Hmodel₂") as "(Hmodel₁ & Hmodel₂)".
+    iSplitL "Hmodel₁".
+    { rewrite list_to_set_disj_app list_to_set_disj_cons right_id comm. iSteps. }
+    iIntros "!> HΦ !>".
+    iSplitR "HΦ"; first iSteps.
+    iIntros "_ Howner {%}".
+
+    wp_smart_apply ws_hub_fifo_notify_spec as "_"; first iSteps.
+    iApply ("HΦ" with "Howner").
+  Qed.
+
+  Lemma ws_hub_fifo_pop'_spec t ι :
+    <<<
+      ws_hub_fifo_inv t ι
+    | ∀∀ vs,
+      ws_hub_fifo_model t vs
+    >>>
+      ws_hub_fifo_pop' t @ ↑ι
+    <<<
+      ∃∃ o,
+      match o with
+      | None =>
+          ws_hub_fifo_model t vs
+      | Some v =>
+          ∃ vs',
+          ⌜vs = {[+v+]} ⊎ vs'⌝ ∗
+          ws_hub_fifo_model t vs'
+      end
+    | RET o;
+      True
+    >>>.
+  Proof.
+    iIntros "%Φ (:inv) HΦ".
+
+    wp_rec. wp_load.
+
+    awp_smart_apply (mpmc_queue_1_pop_spec with "Hqueue_inv").
+    iInv "Hinv" as "(:inv_inner)".
+    iApply (aacc_aupd_commit with "HΦ"); first solve_ndisj. iIntros "%vs (:model)". injection Heq as <-.
+    iDestruct (meta_agree with "Hmeta Hmeta_") as %<-. iClear "Hmeta_".
+    iDestruct (model_agree with "Hmodel₁ Hmodel₂") as %->.
+    iAaccIntro with "Hqueue_model"; first iSteps. iIntros "Hqueue_model".
+    iExists (head ws).
+    destruct ws as [| w ws]; first iSteps.
+    iMod (model_update (list_to_set_disj ws) with "Hmodel₁ Hmodel₂") as "(Hmodel₁ & Hmodel₂)".
+    iSteps.
+  Qed.
+  Lemma ws_hub_fifo_pop_spec t ι i i_ :
+    i = ⁺i_ →
+    <<<
+      ws_hub_fifo_inv t ι ∗
+      ws_hub_fifo_owner t i_
+    | ∀∀ vs,
+      ws_hub_fifo_model t vs
+    >>>
+      ws_hub_fifo_pop t #i @ ↑ι
+    <<<
+      ∃∃ o,
+      match o with
+      | None =>
+          ws_hub_fifo_model t vs
+      | Some v =>
+          ∃ vs',
+          ⌜vs = {[+v+]} ⊎ vs'⌝ ∗
+          ws_hub_fifo_model t vs'
+      end
+    | RET o;
+      ws_hub_fifo_owner t i_
+    >>>.
+  Proof.
+    iIntros (->) "%Φ (Hinv & Howner) HΦ".
+
+    wp_rec.
+    wp_smart_apply (ws_hub_fifo_pop'_spec with "Hinv").
+    iApply (atomic_update_wand with "HΦ"). iIntros "%vs %o HΦ _".
+    iApply ("HΦ" with "Howner").
+  Qed.
+
+  Lemma ws_hub_fifo_steal_until_0_spec P t ι pred :
+    <<<
+      ws_hub_fifo_inv t ι ∗
+      □ WP pred () {{ res,
+        ∃ b,
+        ⌜res = #b⌝ ∗
+        if b then P else True
+      }}
+    | ∀∀ vs,
+      ws_hub_fifo_model t vs
+    >>>
+      ws_hub_fifo_steal_until_0 t pred @ ↑ι
+    <<<
+      ∃∃ o,
+      match o with
+      | None =>
+          ws_hub_fifo_model t vs
+      | Some v =>
+          ∃ vs',
+          ⌜vs = {[+v+]} ⊎ vs'⌝ ∗
+          ws_hub_fifo_model t vs'
+      end
+    | RET o;
+      if o then True else P
+    >>>.
+  Proof.
+    iIntros "%Φ ((:inv) & #Hpred) HΦ".
+    iLöb as "HLöb".
+
+    wp_rec.
+    wp_smart_apply (wp_wand with "Hpred") as (res) "(%b & -> & HP)".
+    destruct b.
+
+    - iApply fupd_wp.
+      iMod "HΦ" as "(%vs & Hmodel & _ & HΦ)".
+      iMod ("HΦ" $! None with "Hmodel") as "HΦ".
+      iSteps.
+
+    - wp_smart_apply domain_yield_spec.
+      awp_smart_apply ws_hub_fifo_pop'_spec; first iSteps.
+      iApply (aacc_aupd with "HΦ"); first done. iIntros "%vs Hmodel".
+      iAaccIntro with "Hmodel"; first iSteps. iIntros ([v |]) "Hmodel".
+
+      + iRight. iExists (Some v). iFrameSteps.
+
+      + iLeft. iFrameSteps.
+  Qed.
+  Lemma ws_hub_fifo_steal_until_spec P t ι i i_ max_round_noyield pred :
+    i = ⁺i_ →
+    (0 ≤ max_round_noyield)%Z →
+    <<<
+      ws_hub_fifo_inv t ι ∗
+      ws_hub_fifo_owner t i_ ∗
+      □ WP pred () {{ res,
+        ∃ b,
+        ⌜res = #b⌝ ∗
+        if b then P else True
+      }}
+    | ∀∀ vs,
+      ws_hub_fifo_model t vs
+    >>>
+      ws_hub_fifo_steal_until t #i #max_round_noyield pred @ ↑ι
+    <<<
+      ∃∃ o,
+      match o with
+      | None =>
+          ws_hub_fifo_model t vs
+      | Some v =>
+          ∃ vs',
+          ⌜vs = {[+v+]} ⊎ vs'⌝ ∗
+          ws_hub_fifo_model t vs'
+      end
+    | RET o;
+      ws_hub_fifo_owner t i_ ∗
+      if o then True else P
+    >>>.
+  Proof.
+    iIntros (-> Hmax_round_noyield) "%Φ (#Hinv & Howner & #Hpred) HΦ".
+
+    wp_rec.
+    wp_smart_apply (ws_hub_fifo_steal_until_0_spec with "[$Hinv $Hpred]").
+    iApply (atomic_update_wand with "HΦ"). iIntros "%vs %o HΦ HP".
+    iApply ("HΦ" with "[$Howner $HP]").
+  Qed.
+
+  Lemma ws_hub_fifo_steal_0_spec t ι :
+    <<<
+      ws_hub_fifo_inv t ι
+    | ∀∀ vs,
+      ws_hub_fifo_model t vs
+    >>>
+      ws_hub_fifo_steal_0 t @ ↑ι
+    <<<
+      ∃∃ o,
+      match o with
+      | None =>
+          ws_hub_fifo_model t vs
+      | Some v =>
+          ∃ vs',
+          ⌜vs = {[+v+]} ⊎ vs'⌝ ∗
+          ws_hub_fifo_model t vs'
+      end
+    | RET o;
+      True
+    >>>.
+  Proof.
+    iIntros "%Φ (:inv) HΦ".
+    iLöb as "HLöb".
+
+    wp_rec. wp_load.
+    wp_smart_apply (waiters_prepare_wait_spec with "Hwaiters_inv") as (waiter) "Hwaiter".
+    wp_smart_apply ws_hub_fifo_killed_spec as ([]) "_"; first iSteps.
+
+    - wp_smart_apply (waiters_cancel_wait_spec with "[$Hwaiters_inv $Hwaiter]") as "_".
+
+      iApply fupd_wp.
+      iMod "HΦ" as "(%vs & Hmodel & _ & HΦ)".
+      iMod ("HΦ" $! None with "Hmodel") as "HΦ".
+      iSteps.
+
+    - wp_load.
+      wp_smart_apply (mpmc_queue_1_is_empty_spec' with "Hqueue_inv") as (b) "_".
+
+      wp_bind (if: _ then _ else _)%E.
+      wp_apply (wp_wand _ _ itype_unit with "[Hwaiter]") as (res) "->".
+      { destruct b; wp_pures.
+        1: wp_apply (waiters_commit_wait_spec with "[$Hwaiters_inv $Hwaiter]").
+        2: wp_apply (waiters_cancel_wait_spec with "[$Hwaiters_inv $Hwaiter]").
+        all: iSteps.
+      }
+
+      awp_smart_apply ws_hub_fifo_pop'_spec; first iSteps.
+      iApply (aacc_aupd with "HΦ"); first done. iIntros "%vs Hmodel".
+      iAaccIntro with "Hmodel"; first iSteps. iIntros ([v |]) "Hmodel".
+
+      + iRight. iExists (Some v). iFrameSteps.
+
+      + iLeft. iFrameSteps.
+  Qed.
+  Lemma ws_hub_fifo_steal_spec t ι i i_ max_round_noyield max_round_yield :
+    i = ⁺i_ →
+    (0 ≤ max_round_noyield)%Z →
+    (0 ≤ max_round_yield)%Z →
+    <<<
+      ws_hub_fifo_inv t ι ∗
+      ws_hub_fifo_owner t i_
+    | ∀∀ vs,
+      ws_hub_fifo_model t vs
+    >>>
+      ws_hub_fifo_steal t #i #max_round_noyield #max_round_yield @ ↑ι
+    <<<
+      ∃∃ o,
+      match o with
+      | None =>
+          ws_hub_fifo_model t vs
+      | Some v =>
+          ∃ vs',
+          ⌜vs = {[+v+]} ⊎ vs'⌝ ∗
+          ws_hub_fifo_model t vs'
+      end
+    | RET o;
+      ws_hub_fifo_owner t i_
+    >>>.
+  Proof.
+    iIntros (-> Hmax_round_noyield Hmax_round_yield) "%Φ (#Hinv & Howner) HΦ".
+
+    wp_rec.
+    wp_smart_apply (ws_hub_fifo_steal_0_spec with "Hinv").
+    iApply (atomic_update_wand with "HΦ"). iIntros "%vs %o HΦ HP".
+    iApply ("HΦ" with "[$Howner $HP]").
+  Qed.
+
+  Lemma ws_hub_fifo_kill_spec t ι :
+    {{{
+      ws_hub_fifo_inv t ι
+    }}}
+      ws_hub_fifo_kill t
+    {{{
+      RET ();
+      True
+    }}}.
+  Proof.
+    iIntros "%Φ (:inv) HΦ".
+
+    wp_rec.
+
+    wp_bind (_ <-{killed} _)%E.
+    iInv "Hinv" as "(:inv_inner)".
+    wp_store.
+    iSplitR "HΦ"; first iSteps.
+    iIntros "!> {%}".
+
+    wp_smart_apply ws_hub_fifo_notify_all_spec as "_"; first iSteps.
+    iSteps.
+  Qed.
+End ws_hub_fifo_G.
+
+#[global] Opaque ws_hub_fifo_inv.
+#[global] Opaque ws_hub_fifo_model.
+#[global] Opaque ws_hub_fifo_owner.
+
+Section ws_hub_fifo_G.
+  Context `{ws_hub_fifo_G : WsHubFifoG Σ}.
+
+  Lemma ws_hub_fifo_pop_steal_until_spec P t ι i i_ max_round_noyield pred :
+    i = ⁺i_ →
+    (0 ≤ max_round_noyield)%Z →
+    <<<
+      ws_hub_fifo_inv t ι ∗
+      ws_hub_fifo_owner t i_ ∗
+      □ WP pred () {{ res,
+        ∃ b,
+        ⌜res = #b⌝ ∗
+        if b then P else True
+      }}
+    | ∀∀ vs,
+      ws_hub_fifo_model t vs
+    >>>
+      ws_hub_fifo_pop_steal_until t #i #max_round_noyield pred @ ↑ι
+    <<<
+      ∃∃ o,
+      match o with
+      | None =>
+          ws_hub_fifo_model t vs
+      | Some v =>
+          ∃ vs',
+          ⌜vs = {[+v+]} ⊎ vs'⌝ ∗
+          ws_hub_fifo_model t vs'
+      end
+    | RET o;
+      ws_hub_fifo_owner t i_ ∗
+      if o then True else P
+    >>>.
+  Proof.
+    iIntros (->) "%Hmax_round_noyield %Φ (#Hinv & Howner & #Hpred) HΦ".
+
+    wp_rec.
+
+    awp_smart_apply (ws_hub_fifo_pop_spec with "[$Hinv $Howner]"); [done.. |].
+    iApply (aacc_aupd with "HΦ"); first done. iIntros "%vs Hmodel".
+    iAaccIntro with "Hmodel"; first iSteps. iIntros ([v |]) "Hmodel !>".
+
+    - iRight. iExists (Some v). iFrame.
+      iIntros "HΦ !> Howner {%}".
+
+      iSpecialize ("HΦ" with "[$Howner]").
+      iSteps.
+
+    - iLeft. iFrame.
+      iIntros "HΦ !> Howner". clear- Hmax_round_noyield.
+
+      wp_smart_apply (ws_hub_fifo_steal_until_spec with "[$Hinv $Howner $Hpred] HΦ"); done.
+  Qed.
+
+  Lemma ws_hub_fifo_pop_steal_spec t ι i i_ max_round_noyield max_round_yield :
+    i = ⁺i_ →
+    (0 ≤ max_round_noyield)%Z →
+    (0 ≤ max_round_yield)%Z →
+    <<<
+      ws_hub_fifo_inv t ι ∗
+      ws_hub_fifo_owner t i_
+    | ∀∀ vs,
+      ws_hub_fifo_model t vs
+    >>>
+      ws_hub_fifo_pop_steal t #i #max_round_noyield #max_round_yield @ ↑ι
+    <<<
+      ∃∃ o,
+      match o with
+      | None =>
+          ws_hub_fifo_model t vs
+      | Some v =>
+          ∃ vs',
+          ⌜vs = {[+v+]} ⊎ vs'⌝ ∗
+          ws_hub_fifo_model t vs'
+      end
+    | RET o;
+      ws_hub_fifo_owner t i_
+    >>>.
+  Proof.
+    iIntros (->) "%Hmax_round_noyield %Hmax_round_yield %Φ (#Hinv & Howner) HΦ".
+
+    wp_rec.
+
+    awp_smart_apply (ws_hub_fifo_pop_spec with "[$Hinv $Howner]"); [done.. |].
+    iApply (aacc_aupd with "HΦ"); first done. iIntros "%vs Hmodel".
+    iAaccIntro with "Hmodel"; first iSteps. iIntros ([v |]) "Hmodel !>".
+
+    - iDestruct "Hmodel" as "(%vs' & -> & Hmodel)".
+      iRight. iExists (Some v). iStep.
+      iIntros "HΦ !> Howner {%}".
+
+      iSpecialize ("HΦ" with "Howner").
+      iSteps.
+
+    - iLeft. iFrame.
+      iIntros "HΦ !> Howner". clear- Hmax_round_noyield Hmax_round_yield.
+
+      wp_smart_apply (ws_hub_fifo_steal_spec with "[$Hinv $Howner] HΦ"); done.
+  Qed.
+End ws_hub_fifo_G.
 
 #[global] Opaque ws_hub_fifo_create.
 #[global] Opaque ws_hub_fifo_killed.
